```agda
{-# OPTIONS --allow-unsolved-metas #-}
module CAS706.A4 where

open import Relation.Binary.PropositionalEquality using (_≡_; refl; cong)
open import Data.Nat using (ℕ; zero; suc; _+_; _<_; _≤_; z≤n; s≤s)
open import Data.Nat.Properties using (m≤m+n)
open import Data.Sum.Base using (_⊎_; inj₁; inj₂)
open import Data.Product.Base
  using (_×_; proj₁; proj₂; ∃-syntax) renaming (_,_ to ⟨_,_⟩)
open import Function.Base using (_∘_)
open import Function.Bundles using (_⇔_; mk⇔)
open import Relation.Nullary.Negation using (¬_)

open import CAS706.part1.Isomorphism using (_≃_)
open _≃_
```

Exercise: SumOfProdImpProdOfSum (10 points)
A disjunct of conjuncts implies a conjunct of disjuncts.

```agda
⊎×-implies-×⊎ : ∀ {A B C D : Set} → (A × B) ⊎ (C × D) → (A ⊎ C) × (B ⊎ D)
⊎×-implies-×⊎ A×B⊎C×D = {!!}
```

Exercise: LTIrrefl (10 points)
 < is irreflexive (never reflexive).
```
¬n<n : ∀ (n : ℕ) → ¬ (n < n)
¬n<n n = {!!}
```

Exercise: ForAllDistProd (10 points)
Show that ∀ distributes over ×.
(The special case of → distributes over × was shown in the Connectives chapter.)
```agda
∀-distrib-× : ∀ {A : Set} {B C : A → Set} →
  (∀ (x : A) → B x × C x) ≃ (∀ (x : A) → B x) × (∀ (x : A) → C x)
∀-distrib-× = {!!}
```

SumForAllImpForAllSum (10 points)
Show that a disjunction of foralls implies a forall of disjunctions.
```agda
⊎∀-implies-∀⊎ : ∀ {A : Set} {B C : A → Set} →
  (∀ (x : A) → B x) ⊎ (∀ (x : A) → C x)  →  ∀ (x : A) → B x ⊎ C x
⊎∀-implies-∀⊎ ∀B⊎∀C = {!!}
```

Exercise: ExistsDistSum (20 points)
Show that existentials distribute over disjunction.
```agda
∃-distrib-⊎ : ∀ {A : Set} {B C : A → Set} →
  ∃[ x ] (B x ⊎ C x) ≃ (∃[ x ] B x) ⊎ (∃[ x ] C x)
∃-distrib-⊎ = {!!}
```

Exercise ExistsProdImpProdExists (10 points)
Show that existentials distribute over ×.
```agda
∃×-implies-×∃ : ∀ {A : Set} {B C : A → Set} →
  ∃[ x ] (B x × C x) → (∃[ x ] B x) × (∃[ x ] C x)
∃×-implies-×∃ = {!!}
```

Exercise: AltLE (30 points)
An alternate definition of y ≤ z.
Hint: mk⇔ and `where` for the pieces. This one is the most difficult of A4.
```agda
∃-≤ : ∀ {y z : ℕ} → ( (y ≤ z) ⇔ ( ∃[ x ] (y + x ≡ z) ) )
∃-≤ = {!!}
```

Exercise: ExistsNegImpNegForAll (1 point)
Existence of negation implies negation of universal.
```agda
∃¬-implies-¬∀ : ∀ {A : Set} {B : A → Set}
  → ∃[ x ] (¬ B x)
    --------------
  → ¬ (∀ x → B x)
∃¬-implies-¬∀ ∃¬B = {!!}
```

The converse cannot be proved in intuitionistic logic.
